src/Core_Erlang_Automated_Exception_Tests.v
@@ -23,13 +23,14 @@ Proof.
 Qed.
 
 Example eval_exception_call :
-  forall {env : Environment} {eff : SideEffectList} {id : nat}, 
-  |env, id, ECall (ELit (Atom "erlang" )) (ELit (Atom "+" )) [ELit (Integer 5); ETuple []], eff|
+  forall {env : Environment}  {eff : SideEffectList} {id : nat}, 
+  |env, [], "", id, ECall (ELit (Atom "erlang" )) (ELit (Atom "+" )) [ELit (Integer 5); ETuple []], eff|
 -e> 
   |id, exception, eff|.
 Proof.
   intros.
   solve.
+  
 Qed.
 
 
@@ -42,11 +43,11 @@ Qed.
 (** DOES NOT COMPPILE IN CORE ERLANG *)
 Example exception_var :
 forall res,
-  ~|[], 0, EVar "X"%string, []|
+  ~|[], [], "", 0, EVar "X"%string, []|
 -e>
   |0, res, []|.
 Proof.
-  unfold not. intros. inversion H. subst. inversion H3.
+  unfold not. intros. inversion H. subst. inversion H5.
 Qed.
 
 Example exception_list_hd_fbs :
@@ -58,7 +59,7 @@ Proof.
 Qed.
 
 Example exception_list_hd :
-  |[], 0, ECons (ECall (ELit (Atom "erlang" )) (ELit (Atom "+" )) [ELit (Integer 5); ETuple []]) (ELit (Atom "error"%string)), []|
+  |[], [], "", 0, ECons (ECall (ELit (Atom "erlang" )) (ELit (Atom "+" )) [ELit (Integer 5); ETuple []]) (ELit (Atom "error"%string)), []|
 -e>
   | 0, exception, []|.
 Proof.
@@ -74,11 +75,12 @@ Proof.
 Qed.
 
 Example exception_list_tl : 
-  |[], 0, ECons (ELit (Atom "error"%string)) (ECons (ECall (ELit (Atom "erlang" )) (ELit (Atom "+" )) [ELit (Integer 5); ETuple []]) (ENil)), []|
+  |[], [], "", 0, ECons (ELit (Atom "error"%string)) (ECons (ECall (ELit (Atom "erlang" )) (ELit (Atom "+" )) [ELit (Integer 5); ETuple []]) (ENil)), []|
 -e> 
   | 0, exception, []|.
 Proof.
-  solve.
+  solve.   
+
 Qed.
 
 Example exception_tuple_fbs : 
@@ -90,11 +92,12 @@ Proof.
 Qed.
 
 Example exception_tuple : 
-  |[], 0, ETuple [ELit (Atom "error"%string) ; ELit (Atom "error"%string); ECall (ELit (Atom "erlang" )) (ELit (Atom "+" )) [ELit (Integer 5); ETuple []]], []|
+  |[], [], "", 0, ETuple [ELit (Atom "error"%string) ; ELit (Atom "error"%string); ECall (ELit (Atom "erlang" )) (ELit (Atom "+" )) [ELit (Integer 5); ETuple []]], []|
 -e>
   | 0, exception, []|.
 Proof.
-  solve.
+  solve. 
+
 Qed.
 
 Example try_eval_fbs : 
@@ -112,7 +115,7 @@ Proof.
 Qed.
 
 Example try_eval : 
-  |[], 0, ETry (ETuple []) ["X"%string]
+  |[], [], "", 0, ETry (ETuple []) ["X"%string]
                (ELit (Atom "ok"%string)) 
                ["Ex1"%string; "Ex2"%string; "Ex3"%string]
                (ELit (Atom "error"%string)) 
@@ -139,7 +142,7 @@ Proof.
 Qed.
 
 Example try_eval_catch : 
-  |[], 0, ETry (ECall (ELit (Atom "erlang" )) (ELit (Atom "+" )) [ELit (Integer 5); ETuple []]) ["X"%string]
+  |[], [], "", 0, ETry (ECall (ELit (Atom "erlang" )) (ELit (Atom "+" )) [ELit (Integer 5); ETuple []]) ["X"%string]
                (ELit (Atom "ok"%string))
                ["Ex1"%string; "Ex2"%string; "Ex3"%string]
                (ELit (Atom "error"%string)) 
@@ -166,7 +169,7 @@ Proof.
 Qed.
 
 Example try_eval_exception : 
-  |[], 0, ETry (ECall (ELit (Atom "erlang" )) (ELit (Atom "+" )) [ELit (Integer 5); ETuple []]) ["X"%string]
+  |[], [], "", 0, ETry (ECall (ELit (Atom "erlang" )) (ELit (Atom "+" )) [ELit (Integer 5); ETuple []]) ["X"%string]
                (ELit (Atom "ok"%string))
                ["Ex1"%string; "Ex2"%string; "Ex3"%string]
                (ECall (ELit (Atom "erlang" )) (ELit (Atom "+" )) [ELit (Integer 5); ETuple []]) 
@@ -175,7 +178,7 @@ Example try_eval_exception :
   |0, exception, []|
 .
 Proof.
-  solve.
+  solve. 
 Qed.
 
 Example try_eval_exception2_fbs : 
@@ -193,7 +196,7 @@ Proof.
 Qed.
 
 Example try_eval_exception2 : 
-  |[], 0, ETry (ETuple []) ["X"%string]
+  |[], [], "", 0, ETry (ETuple []) ["X"%string]
                (ECall (ELit (Atom "erlang" )) (ELit (Atom "+" )) [ELit (Integer 5); ETuple []])
                ["Ex1"%string; "Ex2"%string; "Ex3"%string]
                (ELit (Atom "error"%string))
@@ -202,7 +205,8 @@ Example try_eval_exception2 :
   | 0, exception, []|
 .
 Proof.
-  solve.
+solve.
+
 Qed.
 
 Example eval_case_pat_ex_fbs :
@@ -215,12 +219,12 @@ Proof.
 Qed.
 
 Example eval_case_pat_ex :
-  | [], 0, ECase (ECall (ELit (Atom "erlang" )) (ELit (Atom "+" )) [ELit (Integer 5); ETuple []])
+  |[], [], "", 0, ECase (ECall (ELit (Atom "erlang" )) (ELit (Atom "+" )) [ELit (Integer 5); ETuple []])
                  [([PVar "X"%string], ELit (Atom "true"), ELit (Integer 1))], []|
 -e>
   | 0, exception, []|.
 Proof.
-  solve.
+  solve. 
 Qed.
 
 Example eval_case_clause_ex_fbs :
@@ -235,7 +239,7 @@ Proof.
 Qed.
 
 Example eval_case_clause_ex :
-  | [(inl "Y"%string, VLit (Integer 2))], 0,
+  | [(inl "Y"%string, VLit (Integer 2))], [], "", 0,
      ECase (EVar "Y"%string)
           [([PLit (Integer 1)], ELit (Atom "true"), ELit (Integer 1)); 
            ([PVar "Z"%string], ELit (Atom "false"), ELit (Integer 2))], []|
@@ -254,11 +258,11 @@ Proof.
 Qed.
 
 Example call_eval_body_ex : 
-  |[], 0, ECall (ELit (Atom "erlang" )) (ELit (Atom "+" ))%string [], []|
+  |[], [], "", 0, ECall (ELit (Atom "erlang" )) (ELit (Atom "+" ))%string [], []|
 -e>
   | 0, inr (undef (VLit (Atom "+"))), []|.
 Proof.
-  solve.
+  solve. 
 Qed.
 
 Example call_eval_body_ex2_fbs :
@@ -270,11 +274,11 @@ Proof.
 Qed.
 
 Example call_eval_body_ex2 :
-  |[], 0, ECall (ELit (Atom "erlang" )) (ELit (Atom "+" ))%string [ELit (Integer 5); ETuple []], []|
+  |[], [], "", 0, ECall (ELit (Atom "erlang" )) (ELit (Atom "+" ))%string [ELit (Integer 5); ETuple []], []|
 -e>
   | 0, exception, []|.
 Proof.
-  solve.
+  solve. 
 Qed.
 
 Example call_eval_param_ex_fbs :
@@ -286,11 +290,11 @@ Proof.
 Qed.
 
 Example call_eval_param_ex :
-  |[], 0, ECall (ELit (Atom "erlang" )) (ELit (Atom "+" ))%string [ELit (Integer 5); ECall (ELit (Atom "erlang" )) (ELit (Atom "+" )) [ELit (Integer 5); ETuple []]], []|
+  |[], [], "", 0, ECall (ELit (Atom "erlang" )) (ELit (Atom "+" ))%string [ELit (Integer 5); ECall (ELit (Atom "erlang" )) (ELit (Atom "+" )) [ELit (Integer 5); ETuple []]], []|
 -e>
   |0, exception, []|.
 Proof.
-  solve.
+  solve. 
 Qed.
 
 Example let_eval_exception_params_fbs :
@@ -303,12 +307,12 @@ Proof.
 Qed.
 
 Example let_eval_exception_params :
-  |[], 0, ELet ["X"%string; "Y"%string] 
+  |[], [], "", 0, ELet ["X"%string; "Y"%string] 
                (EValues [ELit (Integer 5); ECall (ELit (Atom "erlang" )) (ELit (Atom "+" )) [ELit (Integer 5); ETuple []]]) (ETuple []), []|
 -e>
   | 0, exception, []|.
 Proof.
-  solve.
+  solve. 
 Qed.
 
 Example let_eval_exception_body_fbs :
@@ -321,12 +325,12 @@ Proof.
 Qed.
 
 Example let_eval_exception_body :
-  |[], 0, ELet ["X"%string; "Y"%string] (EValues [ELit (Integer 5); ELit (Integer 5)])
+  |[], [], "", 0, ELet ["X"%string; "Y"%string] (EValues [ELit (Integer 5); ELit (Integer 5)])
                (ECall (ELit (Atom "erlang" )) (ELit (Atom "+" )) [ELit (Integer 5); ETuple []]), []|
 -e>
   |0, exception, []|.
 Proof.
-  solve.
+  solve. 
 Qed.
 
 Example apply_eval_exception_closure_fbs :
@@ -338,7 +342,7 @@ Proof.
 Qed.
 
 Example apply_eval_exception_closure :
-  |[], 0, EApp (ELit (Integer 4)) [ELit (Integer 5); ELit (Integer 5)], []|
+  |[], [], "", 0, EApp (ELit (Integer 4)) [ELit (Integer 5); ELit (Integer 5)], []|
 -e>
   | 0, inr (badfun (VLit (Integer 4))), []|.
 Proof.
@@ -354,11 +358,11 @@ Proof.
 Qed.
 
 Example apply_eval_exception_closure2 :
-  |[], 0, EApp (ECall (ELit (Atom "erlang" )) (ELit (Atom "+" )) [ELit (Integer 5); ETuple []]) [ELit (Integer 5); ELit (Integer 5)], []|
+  |[], [], "", 0, EApp (ECall (ELit (Atom "erlang" )) (ELit (Atom "+" )) [ELit (Integer 5); ETuple []]) [ELit (Integer 5); ELit (Integer 5)], []|
 -e>
   | 0, exception, []|.
 Proof.
-  solve.
+  solve. 
 Qed.
 
 Example apply_eval_exception_param_fbs :
@@ -371,12 +375,12 @@ Proof.
 Qed.
 
 Example apply_eval_exception_param :
-  |[(inl "X"%string, VClos [] [] 0 [] (ELit (Integer 4)))], 1,
+  |[(inl "X"%string, VClos [] [] 0 [] (ELit (Integer 4)))], [], "", 1,
     EApp (EVar "X"%string) [ECall (ELit (Atom "erlang" )) (ELit (Atom "+" )) [ELit (Integer 5); ETuple []]], []|
 -e>
   |1, exception, []|.
 Proof.
-  solve.
+  solve. 
 Qed.
 
 Example apply_eval_exception_param_count_fbs :
@@ -389,7 +393,7 @@ Proof.
 Qed.
 
 Example apply_eval_exception_param_count :
-  |[(inl "X"%string, VClos [] [] 0 [] (ELit (Integer 4)))], 1,
+  |[(inl "X"%string, VClos [] [] 0 [] (ELit (Integer 4)))], [], "", 1,
    EApp (EVar "X"%string) [ELit (Integer 2)], []|
 -e>
   |1, inr (badarity (VClos [] [] 0 [] (ELit (Integer 4)))), []|.
@@ -407,12 +411,12 @@ Proof.
 Qed.
 
 Example apply_eval_exception_body :
-  |[(inl "X"%string, VClos [] [] 0 [] (ECall (ELit (Atom "erlang" )) (ELit (Atom "+" )) [ELit (Integer 5); ETuple []]))], 1,
+  |[(inl "X"%string, VClos [] [] 0 [] (ECall (ELit (Atom "erlang" )) (ELit (Atom "+" )) [ELit (Integer 5); ETuple []]))], [], "", 1,
    EApp (EVar "X"%string) [], []|
 -e> 
   | 1, exception, []|.
 Proof.
-  solve.
+  solve. 
 Qed.
 
 Example letrec_exception_fbs : 
@@ -424,11 +428,11 @@ Proof.
 Qed.
 
 Example letrec_exception : 
-  |[], 0, ELetRec [(("fun1"%string, 0), ([], ELit (Atom "error"%string)))] (ECall (ELit (Atom "erlang" )) (ELit (Atom "+" )) [ELit (Integer 5); ETuple []]), []|
+  |[], [], "", 0, ELetRec [(("fun1"%string, 0), ([], ELit (Atom "error"%string)))] (ECall (ELit (Atom "erlang" )) (ELit (Atom "+" )) [ELit (Integer 5); ETuple []]), []|
 -e>
   |1, exception, []|.
 Proof.
-  solve.
+  solve. 
 Qed.
 
 Example map_eval_ex_key_fbs :
@@ -443,14 +447,14 @@ Proof.
 Qed.
 
 Example map_eval_ex_key :
-  |[], 0, EMap [(ELit (Atom "error"%string),  ELit (Atom "error"%string)); 
+  |[], [], "", 0, EMap [(ELit (Atom "error"%string),  ELit (Atom "error"%string)); 
                 (ELit (Atom "error"%string), ELit (Atom "error"%string));
                 (ECall (ELit (Atom "erlang" )) (ELit (Atom "+" )) [ELit (Integer 5); ETuple []], ELit (Atom "error"%string));
                 (ELit (Atom "error"%string), ELit (Atom "error"%string))], []|
 -e>
   |0, exception, []|.
 Proof.
-  solve.
+  solve. 
 Qed.
 
 Example map_eval_ex_val_fbs :
@@ -466,14 +470,14 @@ Proof.
 Qed.
 
 Example map_eval_ex_val :
-  |[], 0, EMap [(ELit (Atom "error"%string), ELit (Atom "error"%string)); 
+  |[], [], "", 0, EMap [(ELit (Atom "error"%string), ELit (Atom "error"%string)); 
                 (ELit (Atom "error"%string), ECall (ELit (Atom "erlang" )) (ELit (Atom "+" )) [ELit (Integer 5); ETuple []]);
                 (ELit (Atom "error"%string), ELit (Atom "error"%string));
                 (ELit (Atom "error"%string), ELit (Atom "error"%string))], []|
 -e>
   |0, exception, []|.
 Proof.
-  solve.
+  solve. 
 Qed.
 
 Example seq_eval_ex_1_fbs :
@@ -486,13 +490,13 @@ Proof.
 Qed.
 
 Example seq_eval_ex_1 :
-  | [], 0, ESeq (ECall (ELit (Atom "erlang" )) (ELit (Atom "+" )) [ELit (Integer 5); ETuple []])
+  |[], [], "", 0, ESeq (ECall (ELit (Atom "erlang" )) (ELit (Atom "+" )) [ELit (Integer 5); ETuple []])
                 (ELit (Integer 42))
    , [] |
 -e>
   | 0, exception, [] |.
 Proof.
-  solve.
+  solve. 
 Qed.
 
 Example seq_eval_ex_2_fbs :
@@ -505,13 +509,13 @@ Proof.
 Qed.
 
 Example seq_eval_ex_2 :
-  | [], 0, ESeq (ELit (Integer 42))
+  |[], [], "", 0, ESeq (ELit (Integer 42))
                 (ECall (ELit (Atom "erlang" )) (ELit (Atom "+" )) [ELit (Integer 5); ETuple []])
    , [] |
 -e>
   | 0, exception, [] |.
 Proof.
-  solve.
+  solve. 
 Qed.
 
 Example map_eval_ex_val2_fbs :
@@ -545,7 +549,7 @@ Qed.
 
 
 Example map_eval_ex_val2 :
-  |[], 0, EMap [(ELit (Atom "error"%string), ELit (Atom "error"%string)); 
+  |[], [], "", 0, EMap [(ELit (Atom "error"%string), ELit (Atom "error"%string)); 
                 (ELit (Atom "error"%string), ELit (Atom "error"%string));
                 (ELit (Atom "error"%string), ELit (Atom "error"%string));
                 (ELit (Atom "error"%string), EMap [(ELit (Atom "error"%string), ELit (Atom "error"%string)); 
@@ -570,7 +574,7 @@ Example map_eval_ex_val2 :
 -e>
   |0, exception, []|.
 Proof.
-  solve.
+  solve. 
 Qed.
 
 End Exception_Tests.
